Implement aes128_gcm_compute_iv() for NI and M32

code/aes-gcm/Hacl.AES_128_GCM.M32.fst
@@ -17,30 +17,70 @@ let aes_gcm_ctx_len = 396ul
 
 type aes_gcm_ctx = lbuffer uint64 aes_gcm_ctx_len
 
+val aes128_gcm_compute_iv:
+    ctx: aes_gcm_ctx
+  -> iv_len: size_t
+  -> iv: lbuffer uint8 iv_len ->
+  Stack unit
+  (requires (fun h -> live h ctx /\ live h iv))
+  (ensures (fun h0 _ h1 -> modifies1 ctx h0 h1))
+
+let aes128_gcm_compute_iv ctx iv_len iv =
+  push_frame();
+  if (iv_len =. size 12) then (
+    let tag_iv = create 16ul (u8 0) in
+    let tag_mix = create 16ul (u8 0) in
+    let aes_ctx = sub ctx (size 0) (size 128) in
+    let h0 = ST.get() in
+    loop_nospec #h0 (size 12) tag_iv
+      (fun i -> tag_iv.(i) <- iv.(i));
+    uint_to_bytes_be #U32 (sub tag_iv (size 12) (size 4)) (size 1);
+    aes128_set_nonce aes_ctx tag_iv;
+    aes128_key_block tag_mix aes_ctx;
+    ctx.(394ul) <- uint_from_bytes_le #U64 (sub tag_mix 0ul 8ul);
+    ctx.(395ul) <- uint_from_bytes_le #U64 (sub tag_mix 8ul 8ul);
+    uint_to_bytes_be #U32 (sub tag_iv (size 12) (size 4)) (size 2);
+    aes128_set_nonce aes_ctx tag_iv)
+  else (
+    let gcm_key = create 16ul (u8 0) in
+    let tag_iv = create 16ul (u8 0) in
+    let size_iv = create 16ul (u8 0) in
+    let tag_mix = create 16ul (u8 0) in
+    let aes_ctx = sub ctx (size 0) (size 128) in
+    let gcm_ctx = sub ctx (size 128) (size 266) in
+    uint_to_bytes_be #U64 (sub gcm_key (size 8) (size 8)) gcm_ctx.(size 8);
+    uint_to_bytes_be #U64 (sub gcm_key (size 0) (size 8)) gcm_ctx.(size 9);
+    ghash tag_iv iv_len iv gcm_key;
+    uint_to_bytes_be #U64 (sub size_iv (size 8) (size 8)) (to_u64 (iv_len *. 8ul));
+    let h0 = ST.get() in
+    loop_nospec #h0 (size 16) size_iv
+      (fun i -> size_iv.(i) <- tag_iv.(i) ^. size_iv.(i));
+    ghash tag_iv (size 16) size_iv gcm_key;
+    aes128_set_nonce aes_ctx tag_iv;
+    aes128_key_block tag_mix aes_ctx;
+    ctx.(394ul) <- uint_from_bytes_le #U64 (sub tag_mix 0ul 8ul);
+    ctx.(395ul) <- uint_from_bytes_le #U64 (sub tag_mix 8ul 8ul);
+    uint_to_bytes_be #U32 (sub tag_iv (size 12) (size 4)) ((uint_from_bytes_be #U32 (sub tag_iv (size 12) (size 4))) +. (size 1));
+    aes128_set_nonce aes_ctx tag_iv);
+  pop_frame()
 
 val aes128_gcm_init:
     ctx: aes_gcm_ctx
-  -> key: lbuffer uint8 16ul
-  -> nonce: lbuffer uint8 12ul ->
+  -> key: lbuffer uint8 16ul ->
   Stack unit
-  (requires (fun h -> live h ctx /\ live h key /\ live h nonce))
+  (requires (fun h -> live h ctx /\ live h key))
   (ensures (fun h0 _ h1 -> modifies1 ctx h0 h1))
 
-let aes128_gcm_init ctx key nonce =
+let aes128_gcm_init ctx key =
   push_frame();
   let gcm_key = create 16ul (u8 0) in
-  let tag_mix = create 16ul (u8 0) in
-  let nonce0 = create 12ul (u8 0) in
+  let nonce0 = create 16ul (u8 0) in
   let aes_ctx = sub ctx (size 0) (size 128) in
   let gcm_ctx = sub ctx (size 128) (size 266) in
   admit();
   aes128_init aes_ctx key nonce0;
-  aes128_key_block gcm_key aes_ctx (size 0);
-  aes128_set_nonce aes_ctx nonce;
-  aes128_key_block tag_mix aes_ctx (size 1);
+  aes128_key_block gcm_key aes_ctx;
   gcm_init gcm_ctx gcm_key;
-  ctx.(394ul) <- uint_from_bytes_le #U64 (sub tag_mix 0ul 8ul);
-  ctx.(395ul) <- uint_from_bytes_le #U64 (sub tag_mix 8ul 8ul);
   pop_frame()
 
 
@@ -68,7 +108,7 @@ let aes128_gcm_encrypt ctx len out text aad_len aad =
   let gcm_ctx = sub ctx (size 128) (size 266) in
   let tag_mix = sub ctx (size 394) (size 2) in
   admit();
-  aes128_ctr len cip text aes_ctx (size 2);
+  aes128_ctr len cip text aes_ctx;
   gcm_update_blocks_padded gcm_ctx aad_len aad;
   gcm_update_blocks_padded gcm_ctx len cip;
   uint_to_bytes_be #U64 (sub tmp (size 0) (size 8)) (to_u64 (aad_len *. 8ul));
@@ -81,6 +121,8 @@ let aes128_gcm_encrypt ctx len out text aad_len aad =
   let tmp1 = tmp1 ^. tag_mix.(1ul) in
   uint_to_bytes_le #U64 (sub out len 8ul) tmp0;
   uint_to_bytes_le #U64 (sub out (len +. 8ul) 8ul) tmp1;
+  gcm_ctx.(0ul) <- u64 0;
+  gcm_ctx.(1ul) <- u64 0;
   pop_frame()
 
 
@@ -135,7 +177,7 @@ let aes128_gcm_decrypt ctx len out cipher aad_len aad =
   let res8 = result.(0ul) in
   let r =
     if Lib.RawIntTypes.u8_to_UInt8 res8 = 0uy then (
-      aes128_ctr len out ciphertext aes_ctx (size 2);
+      aes128_ctr len out ciphertext aes_ctx;
       true)
     else (
       let h9 = ST.get () in
